Proved not_free_red_same.

TrTiling.v
@@ -1300,13 +1300,96 @@ Proof.
       forwards* (v''&m3'&Hv''&Hm3'&HR''): IHHR2.
       exists v'' m3'. splits*.
       inverts Hv1. applys* red_args_2.
-      applys* not_is_val_tr. }
+      applys* not_is_val_tr. } }
 Qed.
 
 End TransformationProofs.
 
+(*
+Inductive trm : Type :=
+  | trm_var : var -> trm
+  | trm_val : val -> trm
+  | trm_if : trm -> trm -> trm -> trm
+  | trm_let : bind -> trm -> trm -> trm
+  | trm_app : prim -> list trm -> trm
+  | trm_while : trm -> trm -> trm
+  | trm_for : var -> val -> val -> trm -> trm.
+*)
 
+Inductive free_var (x:var) : trm -> Prop :=
+  | free_var_var :
+      free_var x (trm_var x)
+  | free_var_if : forall t0 t1 t2,
+      free_var x t0 \/ free_var x t1 \/ free_var x t2 ->
+      free_var x (trm_if t0 t1 t2)
+  | free_var_let : forall y t0 t1,
+      free_var x t0 \/ free_var x t1 ->
+      free_var x (trm_let y t0 t1)
+  | free_var_app_1 : forall op t ts,
+      free_var x t ->
+      free_var x (trm_app op (t::ts))
+  | free_var_app_2 : forall op t1 t2 ts,
+      free_var x t1 \/ free_var x t2 ->
+      free_var x (trm_app op (t1::t2::ts))
+  | free_var_while : forall t0 t1,
+      free_var x t0 \/ free_var x t1 ->
+      free_var x (trm_while t0 t1)
+  | free_var_for : forall y a b t,
+      free_var x t ->
+      free_var x (trm_for y a b t).
 
+Theorem not_free_commute_stack : forall C y w2 x w1 S m1 t m2 v,
+  ~ free_var x t ->
+  red C ((x,w1)::(y,w2)::S) m1 t m2 v ->
+  red C ((y,w2)::(x,w1)::S) m1 t m2 v.
+Proof.
+Admitted.
+
+Theorem not_free_red_same : forall C x w S m1 t m2 v,
+  ~ free_var x t ->
+  red C S m1 t m2 v ->
+  red C (Ctx.add x w S) m1 t m2 v.
+Proof.
+  introv Hnf HR. gen x w. induction HR; unfolds Ctx.add;
+  try solve [ constructors* ]; intros.
+  { tests: (x = x0).
+    { forwards*: Hnf. constructors~. }
+    { applys~ red_var. unfolds Ctx.lookup. case_if*.
+      rewrite var_eq_spec in C1. rewrite istrue_isTrue_eq in C1.
+      false*. } }
+  { constructors*.
+    { applys* IHHR1. introv HN. applys Hnf. constructors~. }
+    { applys* IHHR2. introv HN. applys Hnf. constructors. case_if*. } }
+  { constructors*.
+    { applys* IHHR1. introv HN. applys Hnf. constructors~. }
+    { destruct z.
+      { unfolds Ctx.add. applys~ IHHR2. introv HN. 
+        applys Hnf. constructors~. }
+      { unfolds Ctx.add.
+        asserts: (~ free_var x t2).
+        { introv HN. applys~ Hnf. constructors~. }
+        applys~ not_free_commute_stack. } } }
+  { applys~ red_args_1.
+    { applys~ IHHR1. introv HN. applys Hnf. constructors~. }
+    { applys~ IHHR2. introv HN. inverts HN as HN.
+      { inverts HN. }
+      { inverts HN as HN; try solve [ inverts HN ].
+      applys~ Hnf. applys~ free_var_app_2. } } }
+  { applys~ red_args_2.
+    { applys~ IHHR1. introv HN. applys Hnf. applys~ free_var_app_2. }
+    { applys~ IHHR2. introv HN. inverts HN as HN.
+      { inverts HN. }
+      { inverts HN as HN; inverts HN. } } }
+  { applys~ red_var_error. unfolds Ctx.lookup. case_if*.
+    false. applys~ Hnf. rewrite var_eq_spec in C0.
+    rewrite istrue_isTrue_eq in C0. subst. constructors~. }
+  { applys~ red_if_error_not_a_bool.
+    { applys~ IHHR. introv HN. applys~ Hnf. constructors~. }
+    { auto. } }
+  { applys~ red_let_error_let. applys~ IHHR.
+    introv HN. applys~ Hnf. constructors~. }
+  {  }
+Qed.
 
 
 
